code/k256/Hacl.Impl.K256.Point.fst
@@ -89,6 +89,23 @@ let create_point () =
   create (3ul *! 5ul) (u64 0)
 
 
+inline_for_extraction noextract
+val copy_point (out p:point) : Stack unit
+  (requires fun h ->
+    live h out /\ live h p /\ eq_or_disjoint out p /\
+    point_inv h p)
+  (ensures  fun h0 _ h1 -> modifies (loc out) h0 h1 /\
+    point_inv h1 out /\
+    point_eval h1 out == point_eval h0 p)
+
+let copy_point out p =
+  let px, py, pz = getx p, gety p, getz p in
+  let ox, oy, oz = getx out, gety out, getz out in
+  copy_felem ox px;
+  copy_felem oy py;
+  copy_felem oz pz
+
+
 ///  Conversion functions between affine and projective coordinates
 
 inline_for_extraction noextract
